trying to extract blake

code/hash/Hacl.Impl.Blake2s.fst
@@ -37,59 +37,59 @@ let op_String_Access #a #len m b = as_lseq #a #len b m
 /// Helper lemmata
 ///
 
-val lemma_cast_to_u64: x:uint32 -> Lemma
+noextract val lemma_cast_to_u64: x:uint32 -> Lemma
   (requires (True))
   (ensures  (to_u64 #U32 x == u64 (uint_v #U32 x)))
   [SMTPat (to_u64 #U32 x)]
 
 let lemma_cast_to_u64 x = admit()
 
-val lemma_modifies0_is_modifies1: #a0:Type -> #len0:size_nat -> b0:lbuffer a0 len0 -> h0:mem -> h1:mem -> Lemma
+noextract val lemma_modifies0_is_modifies1: #a0:Type -> #len0:size_nat -> b0:lbuffer a0 len0 -> h0:mem -> h1:mem -> Lemma
   (requires (True))
   (ensures  (h0 == h1 ==> modifies1 b0 h0 h1))
 let lemma_modifies0_is_modifies1 #a0 #len0 b0 h0 h1 = admit()
 
 
-val lemma_modifies0_is_modifies2: #a0:Type -> #a1:Type -> #len0:size_nat -> #len1:size_nat -> b0:lbuffer a0 len0 -> b1:lbuffer a1 len1 -> h0:mem -> h1:mem -> Lemma
+noextract val lemma_modifies0_is_modifies2: #a0:Type -> #a1:Type -> #len0:size_nat -> #len1:size_nat -> b0:lbuffer a0 len0 -> b1:lbuffer a1 len1 -> h0:mem -> h1:mem -> Lemma
   (requires (True))
   (ensures  (h0 == h1 ==> modifies2 b0 b1 h0 h1))
 let lemma_modifies0_is_modifies2 #a0 #a1 #len0 #len1 b0 b1 h0 h1 = admit()
 
 
-val lemma_modifies1_is_modifies2: #a0:Type -> #a1:Type -> #len0:size_nat -> #len1:size_nat -> b0:lbuffer a0 len0 -> b1:lbuffer a1 len1 -> h0:mem -> h1:mem -> Lemma
+noextract val lemma_modifies1_is_modifies2: #a0:Type -> #a1:Type -> #len0:size_nat -> #len1:size_nat -> b0:lbuffer a0 len0 -> b1:lbuffer a1 len1 -> h0:mem -> h1:mem -> Lemma
   (requires (True))
   (ensures  (modifies1 b0 h0 h1 ==> modifies2 b0 b1 h0 h1))
 let lemma_modifies1_is_modifies2 #a0 #a1 #len0 #len1 b0 b1 h0 h1 = admit()
 
 
-val lemma_repeati: #a:Type -> n:size_nat -> f:(i:size_nat{i < n}  -> a -> Tot a) -> init:a -> i:size_nat{i < n} -> Lemma
+noextract val lemma_repeati: #a:Type -> n:size_nat -> f:(i:size_nat{i < n}  -> a -> Tot a) -> init:a -> i:size_nat{i < n} -> Lemma
   (requires True)
   (ensures  (f i (repeati #a i f init) == repeati #a (i + 1) f init))
 
 let lemma_repeati #a n f init i = admit()
 
 
-val lemma_repeati_zero: #a:Type -> n:size_nat -> f:(i:size_nat{i < n}  -> a -> Tot a) -> init:a -> Lemma
+noextract val lemma_repeati_zero: #a:Type -> n:size_nat -> f:(i:size_nat{i < n}  -> a -> Tot a) -> init:a -> Lemma
   (requires True)
   (ensures  (init == repeati #a 0 f init))
 
 let lemma_repeati_zero #a n f init = admit()
 
 
-(* val lemma_size_to_uint32_equal_u32_of_v_of_size_t: x:size_t -> Lemma *)
+(* noextract val lemma_size_to_uint32_equal_u32_of_v_of_size_t: x:size_t -> Lemma *)
 (*   (requires True) *)
 (*   (ensures (size_to_uint32 x == u32 (v x))) *)
 (*   [SMTPat (u32 (v x))] *)
 (* let lemma_size_to_uint32_equal_u32_of_v_of_size_t x = admit() *)
 
 
-val lemma_value_mixed_size_addition: x:size_t -> y:size_nat -> Lemma
+noextract val lemma_value_mixed_size_addition: x:size_t -> y:size_nat -> Lemma
   (requires True)
   (ensures (v (x +. (size y)) == v x + y))
   [SMTPat (v (x +. (size y)) == v x + y)]
 let lemma_value_mixed_size_addition x y = admit()
 
-(* val lemma_modifies2_of_subs_is_modifies1: #h0:mem -> #h1:mem -> #a:Type0 -> #len:size_nat -> #pos0:size_nat -> #len0:size_nat{pos0 + len0 < len} -> #pos1:size_nat -> #len1:size_nat{pos1 + len1 <= len} -> buf:lbuffer a len -> sub0:lbuffer a len0 -> sub1:lbuffer a len1 -> *)
+(* noextract val lemma_modifies2_of_subs_is_modifies1: #h0:mem -> #h1:mem -> #a:Type0 -> #len:size_nat -> #pos0:size_nat -> #len0:size_nat{pos0 + len0 < len} -> #pos1:size_nat -> #len1:size_nat{pos1 + len1 <= len} -> buf:lbuffer a len -> sub0:lbuffer a len0 -> sub1:lbuffer a len1 -> *)
 (*   Lemma *)
 (*     (requires (True)) *)
 (*     (ensures  ((modifies2 sub0 sub1 h0 h1 *)
@@ -98,7 +98,7 @@ let lemma_value_mixed_size_addition x y = admit()
 
 (* let lemma_modifies2_of_subs_is_modifies1 #h0 #h1 #a #len #pos0 #len0 #pos1 #len1 buf sub0 sub1 = admit() *)
 
-val lemma_modifies2_trans: #h0:mem -> #h1:mem -> #h2:mem -> #a0:Type0 -> #a1:Type0 -> #len0:size_nat -> #len1:size_nat -> buf0:lbuffer a0 len0 -> buf1:lbuffer a1 len1 ->
+noextract val lemma_modifies2_trans: #h0:mem -> #h1:mem -> #h2:mem -> #a0:Type0 -> #a1:Type0 -> #len0:size_nat -> #len1:size_nat -> buf0:lbuffer a0 len0 -> buf1:lbuffer a1 len1 ->
   Lemma
     (requires (modifies2 buf0 buf1 h0 h1 /\ modifies2 buf0 buf1 h1 h2))
     (ensures  (modifies2 buf0 buf1 h0 h2))
@@ -107,6 +107,7 @@ let lemma_modifies2_trans #h0 #h1 #h2 #a0 #a1 #len0 #len1 buf0 buf1 = admit()
 
 
 (* Functions to add to the libraries *)
+[@ Substitute]
 val update_sub: #a:Type0 -> #len:size_nat -> #xlen:size_nat -> i:lbuffer a len -> start:size_t -> n:size_t{v start + v n <= len /\ v n == xlen} -> x:lbuffer a xlen ->
   Stack unit
     (requires (fun h -> live h i /\ live h x))
@@ -140,7 +141,7 @@ noeq type state = {
 }
 
 
-val state_invariant: h:mem -> st:state -> Type0
+noextract val state_invariant: h:mem -> st:state -> Type0
 let state_invariant h st =
     live h st.hash /\ live h st.const_iv /\ live h st.const_sigma
   /\ disjoint st.hash st.const_iv /\ disjoint st.const_iv st.hash
@@ -386,7 +387,6 @@ let blake2_compress s m offset flag const_iv const_sigma =
     blake2_compress2 wv m const_sigma;
     blake2_compress3 wv s const_sigma)
 
-
 val blake2s_update_block:
     st:state
   -> dd_prev:size_t
@@ -570,8 +570,6 @@ let blake2s_finish #vnn output s nn =
     uints_to_bytes_le full s.hash;
     update_sub output (size 0) nn full)
 
-
-
 val blake2s:
     #vll: size_nat
   -> #vkk: size_nat
@@ -594,20 +592,22 @@ let blake2s #vll #vkk #vnn output d ll kk k nn =
   let rem = ll %. (size Spec.size_block) in
   let nblocks = ll /. (size Spec.size_block) in
   let blocks = sub #uint8 #vll #(v nblocks * Spec.size_block) d (size 0) (nblocks *. (size Spec.size_block)) in
-  let last = sub d (nblocks *. (size Spec.size_block)) rem in
+  let last = sub #_ #_ #(v rem) d (nblocks *. (size Spec.size_block)) rem in
   let st = blake2s_mkstate () in
   if  ll =. (size 0) && kk =. (size 0) then begin
     let h0 = ST.get () in
-    alloc1 #h0 (size Spec.size_block) (u8 0) output
+    alloc1 #h0 #_ #_ #_ #Spec.size_block #vnn (size Spec.size_block) (u8 0) output
     (fun h -> (fun _ r -> True))
     (fun data ->
       let h0 = ST.get () in
       blake2s_init #vkk st k kk nn;
       blake2s_update_last #(v rem) st ll data (size Spec.size_block) fk;
-      blake2s_finish #vnn output st nn) end
+      blake2s_finish #vnn output st nn
+      ) end
   else
     blake2s_init #vkk st k kk nn;
     let nprev = if kk =. (size 0) then (size 0) else (size 1) in
-    blake2s_update_multi st nprev nblocks d;
+    blake2s_update_multi st (size 0) nblocks d;
     blake2s_update_last #(v rem) st ll last rem fk;
     blake2s_finish #vnn output st nn
+
